motivating example now works fully

theories/iris/examples/effects/coroutines_client.v
@@ -4,8 +4,9 @@ From iris.program_logic Require Import language.
 From iris.proofmode Require Import base tactics classes.
 From iris.base_logic Require Export gen_heap ghost_map proph_map.
 From iris.base_logic.lib Require Export fancy_updates.
+From iris.program_logic Require Import adequacy.
 From iris.bi Require Export weakestpre.
-From iris.algebra Require Import auth excl.
+From iris.algebra Require Import excl agree csum.
 From Wasm Require Import type_checker_reflects_typing.
 From Wasm.iris.rules Require Export iris_rules iris_example_helper.
 From Wasm.iris.host Require Export iris_host.
@@ -17,25 +18,43 @@ Set Implicit Arguments.
 Unset Strict Implicit.
 Unset Printing Implicit Defensive.
 
+(*
+Class natG Σ := NAtG {
+                    nat_genG :: ghost_mapG Σ unit nat
+                  } .
+Notation "γ ○↪ v" := (ghost_map_elem γ tt (DfracOwn 1) v%V) (at level 20).
+Notation "γ ●↪ v" := (ghost_map_auth γ 1 (<[ tt := (v : nat) ]> ∅)) (at level 20).
+ *)
+Definition one_shotR := csumR (exclR unitO) (agreeR unitO).
+Definition Pending : one_shotR := Cinl (Excl ()).
+Definition Shot : one_shotR := Cinr (to_agree ()).
+
+Class one_shotG Σ := { #[local] one_shot_inG :: inG Σ one_shotR }.
+
+Definition one_shotΣ : gFunctors := #[GFunctor one_shotR].
+Global Instance subG_one_shotΣ {Σ} : subG one_shotΣ Σ → one_shotG Σ.
+Proof. solve_inG. Qed.
+
+
+
 Section coroutines_client_functions.
 
-  Context `{!wasmG Σ, !hvisG Σ, !hmsG Σ, !hasG Σ}.
-  Context `{!inG Σ (one_shotR unitO)}.
+  Context `{!wasmG Σ, !hvisG Σ, !hmsG Σ, !hasG Σ, !one_shotG Σ}.
 
    Definition f1 :=
      [ BI_const (xx 1);
-       BI_set_global 0;
+       BI_set_global 2;
        BI_call 0;
        BI_const (xx 1);
-       BI_set_global 1
+       BI_set_global 3
      ].
 
    Definition f2 :=
-     [ BI_get_global 1;
-       BI_set_global 2;
+     [ BI_get_global 3;
+       BI_set_global 0;
        BI_call 0;
-       BI_get_global 0;
-       BI_set_global 3
+       BI_get_global 2;
+       BI_set_global 1
      ].
 
    Definition main :=
@@ -48,52 +67,48 @@ Section coroutines_client_functions.
 
    Definition wgpt a b :=
      N.of_nat a ↦[wg] {| g_mut := MUT_mut ; g_val := xx b |}.
-   Definition wgpt_half a b :=
-     N.of_nat a ↦[wg]{ DfracOwn (1/2)%Qp } {| g_mut := MUT_mut ; g_val := xx b |}.
    
-   Definition P1 addrx : iProp Σ :=
-     wgpt_half addrx 0.
+   Definition P1 : iProp Σ := True.
 
-   Definition Q1 addrx : iProp Σ :=
-     wgpt_half addrx 1.
+   Definition Q1 γx γy : iProp Σ := own γx Shot ∗ own γy Shot.
 
-   Definition P2 addra addrb : iProp Σ :=
+   Definition P2 addra addrb: iProp Σ :=
      ∃ a b, wgpt addra a ∗ wgpt addrb b. 
 
-   Definition Q2 addra addrb : iProp Σ :=
+   Definition Q2 addra addrb: iProp Σ :=
      ∃ a b, wgpt addra a ∗ wgpt addrb b ∗ ⌜ a = 1 -> b = 1 ⌝ .
 
-   Definition I addrx addry : iProp Σ :=
-     (wgpt_half addrx 0 ∗ wgpt addry 0) ∨
-       (wgpt_half addrx 1 ∗ wgpt addry 0) ∨
-       (wgpt_half addrx 1 ∗ wgpt addry 1).
+   Definition I addrx addry γx γy : iProp Σ :=
+     (wgpt addrx 0 ∗ wgpt addry 0 ∗ own γx Pending ∗ own γy Pending) ∨
+       (wgpt addrx 1 ∗ wgpt addry 0 ∗ own γx Shot ∗ own γy Pending) ∨
+       (wgpt addrx 1 ∗ wgpt addry 1 ∗ own γx Shot ∗ own γy Shot).
 
-   Definition spec_f1 f Ψ addr_f1 cl_f1 addrx addry addr_yield cl_yield: iProp Σ :=
+   Definition spec_f1 f Ψ γx γy addr_f1 cl_f1 addrx addry addr_yield cl_yield: iProp Σ :=
      □ (N.of_nat addr_f1 ↦[wf] cl_f1 -∗
         N.of_nat addr_yield ↦[wf] cl_yield -∗
-         P1 addrx -∗
-         I addrx addry -∗
+         P1 -∗
+         I addrx addry γx γy -∗
               EWP [AI_invoke addr_f1] UNDER f <| Ψ |> {{ v; f' ,
                   ⌜ v = immV [] ⌝ ∗
                   ⌜ f' = f ⌝ ∗
                   N.of_nat addr_f1 ↦[wf] cl_f1 ∗
                   N.of_nat addr_yield ↦[wf] cl_yield ∗
-                  Q1 addrx ∗
-                  I addrx addry
+                  Q1 γx γy ∗
+                  I addrx addry γx γy
        }})%I.
    
-   Definition spec_f2 f Ψ addr_f2 cl_f2 addrx addry addra addrb addr_yield cl_yield: iProp Σ :=
+   Definition spec_f2 f Ψ γx γy addr_f2 cl_f2 addrx addry addra addrb addr_yield cl_yield: iProp Σ :=
      □ (N.of_nat addr_f2 ↦[wf] cl_f2 -∗
           N.of_nat addr_yield ↦[wf] cl_yield -∗
           P2 addra addrb -∗
-          I addrx addry -∗
+          I addrx addry γx γy -∗
              EWP [AI_invoke addr_f2] UNDER f <| Ψ |> {{ v; f' ,
                 ⌜ v = immV [] ⌝ ∗
                 ⌜ f' = f ⌝ ∗
                 N.of_nat addr_f2 ↦[wf] cl_f2 ∗
                 N.of_nat addr_yield ↦[wf] cl_yield ∗
                 Q2 addra addrb ∗
-                I addrx addry }})%I.
+                I addrx addry γx γy }})%I.
 
    Definition spec_main f Ψ addr_main cl_main addrx addry addra addrb addr_yield cl_yield addr_par cl_par addr_f1 cl_f1 addr_f2 cl_f2: iProp Σ :=
      □ (N.of_nat addr_main ↦[wf] cl_main -∗
@@ -118,13 +133,13 @@ Section coroutines_client_functions.
       inst_funcs := [ addr_yield; addr_par; addr_f1; addr_f2; addr_main ] ;
       inst_tab := [];
       inst_memory := [];
-      inst_globs := [addrx; addry; addra; addrb];
+      inst_globs := [addra; addrb; addrx; addry];
       inst_tags := [] |}.
    
-   Lemma spec_f1_proof f Ψ addr_f1 cl_f1 addrx addry addr_yield cl_yield addr_par addr_f2 addr_main addra addrb :
+   Lemma spec_f1_proof f Ψ γx γy addr_f1 cl_f1 addrx addry addr_yield cl_yield addr_par addr_f2 addr_main addra addrb :
      cl_f1 = FC_func_native (client_inst addr_yield addr_par addr_f1 addr_f2 addr_main addrx addry addra addrb) emptyt [] f1 ->
-     yield_spec addr_yield cl_yield Ψ (I addrx addry)
-       ⊢ spec_f1 f Ψ addr_f1 cl_f1 addrx addry addr_yield cl_yield.
+     yield_spec addr_yield cl_yield Ψ (I addrx addry γx γy)
+       ⊢ spec_f1 f Ψ γx γy addr_f1 cl_f1 addrx addry addr_yield cl_yield.
    Proof.
      iIntros (->) "#Hyield !> Hwf1 Hwfyield HP1 HI".
      rewrite - (app_nil_l [AI_invoke addr_f1]).
@@ -143,186 +158,215 @@ Section coroutines_client_functions.
          instantiate (5 := []).
          rewrite /lfilled /lfill /= app_nil_r //. }
      rewrite separate2.
+     iAssert (∃ x, wgpt addrx x ∗ (own γx Pending ∨ own γx Shot) ∗ ∃ y, wgpt addry y ∗ (⌜ y = 0 ⌝ ∗ own γy Pending ∨ ⌜ y = 1 ⌝ ∗ own γy Shot))%I with "[HI]" as "(%x & Hx & Htokx & %y & Hy & Htoky)".
+     { iDestruct "HI" as "[(Hx & Hy & Htokx & Htoky) | [(Hx & Hy & Htokx & Htoky) | (Hx & Hy & Htokx & Htoky)]]".
+       all: iFrame.
+       1-2: by iLeft; iFrame.
+       by iRight; iFrame.
+     } 
      iApply ewp_seq.
      done.
      iSplitR; last first.
-     iAssert (wgpt addrx 0 ∗ wgpt addry 0)%I with "[HI HP1]" as "[Hx Hy]".
-     { iDestruct "HI" as "[[Hx Hy] | [[Hx Hy] | [Hx Hy]]]".
-       iFrame.
-       all: iDestruct (pointsto_agree with "Hx HP1") as "%Habs" => //. } 
      iSplitL "Hx".
-     iApply (ewp_set_global with "[] Hx").
-     done.
+     iApply (ewp_set_global with "[] Hx"); first done.
      auto_instantiate.
      2: by iIntros (?) "[[% _] _]".
      iIntros (??) "[[-> ->] Hx]".
      iSimpl.
+     iApply fupd_ewp.
+     iAssert (|={⊤}=> own γx Shot)%I with "[Htokx]" as "Htokx".
+     { iDestruct "Htokx" as "[Htokx | Htokx]"; last done.
+       iMod (own_update with "Htokx") as "Htokx"; last done.
+       apply cmra_update_exclusive. done. }
+     iMod "Htokx" as "#Htokx". 
+     iModIntro.
      rewrite (separate1 (AI_basic _)).
-     iApply ewp_seq.
-     done.
+     iApply ewp_seq; first done.
      iSplitR; last first.
      simpl.
-     iDestruct "Hx" as "[Hx1 Hx2]".
-     iSplitR "Hx2".
-     iApply ewp_call.
-     done.
-     iApply ("Hyield" with "[Hx1 Hy] Hwfyield").
-     simpl.
-     iRight. iLeft. iFrame.
+     iSplitL.
+     iApply ewp_call; first done.
+     iApply ("Hyield" with "[Hx Hy Htoky] Hwfyield").
+     iRight.
+     iDestruct "Htoky" as "[[-> Htoky] | [-> Htoky]]"; iFrame.
+     by iLeft; iFrame. by iRight; iFrame.
+     2: by iIntros (?) "[% _]".
      iIntros (??) "(-> & -> & HI & Hwfyield)".
      iSimpl.
-     iAssert (wgpt addrx 1 ∗ ∃ i, wgpt addry i)%I with "[HI Hx2]" as "(Hx & %i & Hy)".
+     iAssert (wgpt addrx 1 ∗ ∃ i, wgpt addry i ∗ (own γy Pending ∨ own γy Shot))%I with "[HI]" as "(Hx & %i & Hy & Htoky)".
 
-     { iDestruct "HI" as "[[Hx Hy] | [[Hx Hy] | [Hx Hy]]]".
-       iDestruct (pointsto_agree with "Hx Hx2") as %Habs => //.
-       all: iFrame. }
+     { iDestruct "HI" as "[(Hx & Hy & Htokx2 & Htoky) | [(Hx & Hy & _ & Htoky) | (Hx & Hy & _ & Htoky)]]".
+       iDestruct (own_valid_2 with "Htokx Htokx2") as "%Habs".
+       done.
+       all: iFrame. } 
      iApply (ewp_wand with "[Hy]").
      iApply (ewp_set_global with "[] Hy").
      done.
      auto_instantiate.
-     2: by iIntros (?) "[% _]".
      iIntros (??) "[[-> ->] Hy]".
      simpl.
      iIntros (LI HLI).
      move/lfilledP in HLI; inversion HLI; subst.
      inversion H8; subst.
      iSimpl.
+     iApply fupd_ewp.
+     iAssert (|={⊤}=> own γy Shot)%I with "[Htoky]" as "Htoky".
+     { iDestruct "Htoky" as "[Htoky | Htoky]"; last done.
+       iMod (own_update with "Htoky") as "Htoky"; last done.
+       apply cmra_update_exclusive. done. }
+     iMod "Htoky" as "#Htoky".
+     iModIntro.
      iApply ewp_label_value.
      done.
      instantiate (1 := λ v f,  (⌜ v = immV _ ⌝ ∗ ⌜ f = Build_frame _ _ ⌝ ∗ _)%I).
      iSplitR; first done.
      iSplitR; first done.
-     iCombine "Hwfyield Hx Hy" as "H".
+     iCombine "Hwfyield Hx Hy Htokx Htoky" as "H".
      iExact "H".
-     iIntros (??) "(-> & -> & Hwfyield & Hx & Hy)".
+     iIntros (??) "(-> & -> & Hwfyield & Hx & Hy & #Htokx & #Htoky)".
      iApply ewp_frame_value.
      done. done.
      iSplit; first done.
      iSplit; first done.
      iFrame.
-     iDestruct "Hx" as "[Hx1 Hx2]".
-     iFrame.
-     iRight. iRight.
+     iFrame "Htokx Htoky".
+     iRight; iRight.
      iFrame.
      iIntros (?) "[% _]" => //.
    Qed. 
      
-   Lemma spec_f2_proof f Ψ addr_f2 cl_f2 addrx addry addr_yield cl_yield addr_par addr_f1 addr_main addra addrb :
+   Lemma spec_f2_proof f Ψ addr_f2 cl_f2 addrx addry γx γy addr_yield cl_yield addr_par addr_f1 addr_main addra addrb :
      cl_f2 = FC_func_native (client_inst addr_yield addr_par addr_f1 addr_f2 addr_main addrx addry addra addrb) emptyt [] f2 ->
-     yield_spec addr_yield cl_yield Ψ (I addrx addry)
-       ⊢ spec_f2 f Ψ addr_f2 cl_f2 addrx addry addra addrb addr_yield cl_yield.
+     yield_spec addr_yield cl_yield Ψ (I addrx addry γx γy)
+       ⊢ spec_f2 f Ψ γx γy addr_f2 cl_f2 addrx addry addra addrb addr_yield cl_yield.
    Proof.
      iIntros (->) "#Hyield !> Hwf2 Hwfyield HP2 HI".
      iDestruct "HP2" as (a b) "[Ha Hb]".
-     iDestruct "HI" as "[[Hx Hy] | [[Hx Hy] | [Hx Hy]]]".
-     - (* Case 1 *) 
-       rewrite - (app_nil_l [AI_invoke addr_f2]).
-       iApply (ewp_invoke_native with "Hwf2").
-       done. done. done.
-       iIntros "!> Hwf2".
-       iApply ewp_frame_bind.
-       done. done.
-       iSplitR; last first.
-       iSplitR "Hwf2".
-       rewrite -(app_nil_l [AI_basic _]).
-       iApply ewp_block.
-       done. done. done. done.
-       iApply (ewp_label_bind with "[-]").
-       2:{ iPureIntro.
-           instantiate (5 := []).
-           rewrite /lfilled /lfill /= app_nil_r //. }
-       rewrite (separate1 (AI_basic _)).
-       iApply ewp_seq.
-       done.
-       iSplitR; last first.
-       iSplitL "Hy".
-       iApply (ewp_get_global with "[] Hy").
-       done. done.
-       iSimpl.
-       auto_instantiate.
-       2: by iIntros (?) "[[% _] _]".
-       iIntros (??) "[[->->] Hy]".
-       iSimpl.
-       rewrite separate2.
-       iApply ewp_seq.
-       done.
-       iSplitR; last first.
-       iSplitL "Ha".
-       iApply (ewp_set_global with "[] Ha").
-       done.
-       auto_instantiate.
-       2: by iIntros (?) "[[% _] _]".
-       iIntros (??) "[[-> ->] Ha]".
-       iSimpl.
-       rewrite (separate1 (AI_basic _)).
-       iApply ewp_seq.
-       done.
-       iAssert (I addrx addry)%I with "[Hx Hy]" as "HI".
-       by iLeft; iFrame.
-       iSplitR; last first.
-       iSplitL "HI Hwfyield".
-       iApply ewp_call.
-       done.
-       iApply ("Hyield" with "HI Hwfyield").
-       2: by iIntros (?) "[% _]".
-       iIntros (??) "(-> & -> & HI & Hwfyield)".
-       iDestruct "HI" as "[[Hx Hy] | [[ Hx Hy ] | [Hx Hy]]]".
-
-       iSimpl.
-        rewrite (separate1 (AI_basic _)).
-        iApply ewp_seq.
-        try done.
-        iSplitR; last first.
-        try iSplitL "Hx".
-        try iApply (ewp_get_global with "[] Hx").
-        try done.
-        try by auto_instantiate.
-        try by iIntros (?) "[[% _] _]".
-        iIntros (??) "[[-> ->] Hx]".
-        iSimpl.
-        iApply (ewp_wand with "[Hb]").
-        try iApply (ewp_set_global with "[] Hb").
-        try done.
-        try auto_instantiate.
-        iIntros (??) "[[-> ->] Hb]".
-        iIntros (LI HLI).
-        move/lfilledP in HLI; inversion HLI; subst.
-        inversion H8; subst.
-        iApply ewp_label_value.
-        try done.
-       instantiate (1 := λ v f, (⌜ v = immV _ ⌝ ∗ ⌜ f = Build_frame _ _ ⌝ ∗ _ ∗ (_ ∨ _ ∨ _ ∨ _ ∨ _ ∨ _ ∨ _ ∨ _ ∨ _))%I).
-        iSplit; first done.
-        iSplit; first done.
-        iSplitL "Hwfyield"; first iExact "Hwfyield".
-        iCombine "Ha Hb Hx Hy" as "H".
-       iLeft; iExact "H".
-        iRight.
-       iLeft; iExact "H".
-        iRight.
-       iLeft; iExact "H".
-        iRight.
-       iLeft; iExact "H".
-        iRight.
-       iLeft; iExact "H".
-        iRight.
-       iLeft; iExact "H".
-        iRight.
-       iLeft; iExact "H".
-        iRight.
-       iLeft; iExact "H".
-       iRight.
-       iExact "H".
-     }
+     iAssert (∃ y, wgpt addry y ∗ (⌜ y = 1 ⌝ ∗ own γy Shot ∗ wgpt addrx 1 ∗ own γx Shot ∨ ⌜ y = 0 ⌝ ∗ own γy Pending ∗ ∃ x, wgpt addrx x ∗ (⌜ x = 0 ⌝ ∗ own γx Pending ∨ ⌜ x = 1 ⌝ ∗ own γx Shot)))%I with "[HI]" as "(%y & Hy & Htoky)".
+     { iDestruct "HI" as "[(Hx & Hy & Htokx & Htoky) | [(Hx & Hy & Htokx & Htoky) | (Hx & Hy & Htokx & Htoky)]]".
+       all: iFrame.
+       - iRight. iFrame. iSplit; first done.
+         by iLeft; iFrame.
+       - iRight; iFrame. iSplit; first done.
+         by iRight; iFrame.
+       - by iLeft; iFrame. } 
+     rewrite - (app_nil_l [AI_invoke addr_f2]).
+     iApply (ewp_invoke_native with "Hwf2").
+     done. done. done.
+     iIntros "!> Hwf2".
+     iApply ewp_frame_bind.
+     done. done.
+     iSplitR; last first.
+     iSplitR "Hwf2".
+     rewrite -(app_nil_l [AI_basic _]).
+     iApply ewp_block.
+     done. done. done. done.
+     iApply (ewp_label_bind with "[-]").
+     2:{ iPureIntro.
+         instantiate (5 := []).
+         rewrite /lfilled /lfill /= app_nil_r //. }
+     rewrite (separate1 (AI_basic _)).
+     iApply ewp_seq.
+     done.
+     iSplitR; last first.
+     iSplitL "Hy".
+     iApply (ewp_get_global with "[] Hy").
+     done. done.
+     iSimpl.
+     auto_instantiate.
+     2: by iIntros (?) "[[% _] _]".
+     iIntros (??) "[[->->] Hy]".
+     iSimpl.
+     rewrite separate2.
+     iApply ewp_seq.
+     done.
+     iSplitR; last first.
+     iSplitL "Ha".
+     iApply (ewp_set_global with "[] Ha").
+     done.
+     auto_instantiate.
+     2: by iIntros (?) "[[% _] _]".
+     iIntros (??) "[[-> ->] Ha]".
+     iSimpl.
+     rewrite (separate1 (AI_basic _)).
+     iApply ewp_seq.
+     done.
+     iAssert (I addrx addry γx γy ∗ (⌜ y = 1 ⌝ ∗ own γy Shot ∗ own γx Shot ∨ ⌜ y = 0 ⌝))%I with "[Hy Htoky]" as "[HI #Htoky]".
+     { iDestruct "Htoky" as "[(-> & #Htoky & Hx & #Htokx) | (-> & Htoky & %x & Hx & [[-> Htokx] | [-> Htokx]])]".
+       iSplitL; last by iLeft; iFrame "Htokx Htoky".
+       by iRight; iRight; iFrame "Htokx Htoky Hx Hy".
+       all: iSplitL; last by iRight.
+       iLeft; by iFrame.
+       iRight; iLeft; by iFrame. } 
+     iSplitR; last first.
+     iSplitL "HI Hwfyield".
+     iApply ewp_call.
+     done.
+     iApply ("Hyield" with "HI Hwfyield").
      2: by iIntros (?) "[% _]".
-     iIntros (??) "(-> & -> & Hwfyield & H)".
+     iIntros (??) "(-> & -> & HI & Hwfyield)".
+     iAssert (∃ x, wgpt addrx x ∗ (⌜ x = 0 ⌝ ∗ ⌜ y = 0 ⌝ ∗ own γx Pending ∗ wgpt addry 0 ∗ own γy Pending ∨ ⌜ x = 1 ⌝ ∗ own γx Shot ∗ ∃ y, wgpt addry y ∗ (⌜ y = 0 ⌝ ∗ own γy Pending ∨ ⌜ y = 1 ⌝ ∗ own γy Shot)))%I with "[HI]" as "(%x & Hx & Htokx)".
+     { iDestruct "HI" as "[(Hx & Hy & Htokx & Htoky') | [(Hx & Hy & Htokx & Htoky') | (Hx & Hy & Htokx & Htoky')]]".
+       all: iFrame.
+       - iLeft.
+         iDestruct "Htoky" as "[(-> & Htoky & Htokx') | ->]".
+         iDestruct (own_valid_2 with "Htokx Htokx'") as "%Habs".
+         done.
+         iFrame. done.
+       - iRight. iFrame. iSplit; first done. by iLeft; iFrame.
+       - iRight. iFrame. iSplit; first done. by iRight; iFrame. } 
+     iSimpl.
+     rewrite (separate1 (AI_basic _)).
+     iApply ewp_seq.
+     done.
+     iSplitR; last first.
+     iSplitL "Hx".
+     iApply (ewp_get_global with "[] Hx").
+     done. done.
+     by auto_instantiate.
+     2: by iIntros (?) "[[% _] _]".
+     iIntros (??) "[[-> ->] Hx]".
+     iSimpl.
+     iApply (ewp_wand with "[Hb]").
+     iApply (ewp_set_global with "[] Hb").
+     done.
+     auto_instantiate.
+     iIntros (??) "[[-> ->] Hb]".
+     iIntros (LI HLI).
+     move/lfilledP in HLI; inversion HLI; subst.
+     inversion H8; subst.
+     iApply ewp_label_value.
+     done.
+     instantiate (1 := λ v f, (⌜ v = immV [] ⌝ ∗ ⌜ f = Build_frame [] _ ⌝ ∗ ∃ x, N.of_nat addra↦[wg] {| g_mut := MUT_mut; g_val := xx y |} ∗
+        N.of_nat addrb↦[wg] {| g_mut := MUT_mut; g_val := xx x |} ∗
+        N.of_nat addrx↦[wg] {| g_mut := MUT_mut; g_val := xx x |} ∗
+        (⌜x = 0⌝ ∗ ⌜y = 0⌝ ∗ own γx Pending ∗ wgpt addry 0 ∗ 
+         own γy Pending ∨ ⌜x = 1⌝ ∗ own γx Shot ∗
+         ∃ y0 : Z, wgpt addry y0 ∗
+           (⌜y0 = 0⌝ ∗ own γy Pending ∨ ⌜y0 = 1⌝ ∗ own γy Shot)) ∗
+        N.of_nat addr_yield↦[wf]cl_yield)%I).
+     iSplit; first done.
+     iSplit; first done.
+     iCombine "Ha Hb Hx Htokx Hwfyield" as "H".
+     simpl. iNext. iExists x. done.
+     2: by iIntros (?) "[% _]".
+     iIntros (??) "(-> & -> & %x & Ha & Hb & Hx & Htokx & Hwfyield)".
      iApply ewp_frame_value.
      done. done.
      iSplit; first done.
      iSplit; first done.
      iFrame.
-     iDestruct "H" as "[ (Ha & Hb & Hx & Hy) | [ (Ha & Hb & Hx & Hy) | [ (Ha & Hb & Hx & Hy) | [ (Ha & Hb & Hx & Hy) | [ (Ha & Hb & Hx & Hy) | [ (Ha & Hb & Hx & Hy) | [ (Ha & Hb & Hx & Hy) | [ (Ha & Hb & Hx & Hy) | (Ha & Hb & Hx & Hy) ]]]]]]]]".
-     all: iFrame.
-     all: iSplit; first try done.
+     iNext.
+     iSplit.
+     { (* the implication *)
+       iDestruct "Htokx" as "[(-> & -> & _) | [-> _]]".
+       all: done. }
+     (* reconstructing the invariant *)
+     iDestruct "Htokx" as "[(-> & -> & Htokx & Hy & Htoky) | (-> & Htokx & %y' & Hy & [[-> Htoky] | [-> Htoky]])]".
+     - iLeft. iFrame.
+     - iRight. iLeft. iFrame.
+     - iRight. iRight. iFrame. 
+   Qed. 
        
        
 
@@ -333,7 +377,7 @@ End coroutines_client_functions.
 
 Section coroutines_client_module.
 
-  Context `{!wasmG Σ, !hvisG Σ, !hmsG Σ, !hasG Σ}.
+  Context `{!wasmG Σ, !hvisG Σ, !hmsG Σ, !hasG Σ, !one_shotG Σ}.
 
   Definition client_module :=
     {|
@@ -361,11 +405,11 @@ Section coroutines_client_module.
         {| modglob_type := {| tg_mut := MUT_mut ; tg_t := T_i32 |} ;
           modglob_init := [BI_const (xx 0)] |};
         {| modglob_type := {| tg_mut := MUT_mut ; tg_t := T_i32 |} ;
-          modglob_init := [BI_const (xx 0)] |};
+          modglob_init := [BI_const (xx 0)] |} (* ;
         {| modglob_type := {| tg_mut := MUT_mut ; tg_t := T_i32 |} ;
           modglob_init := [BI_const (xx 0)] |};
         {| modglob_type := {| tg_mut := MUT_mut ; tg_t := T_i32 |} ;
-          modglob_init := [BI_const (xx 0)] |}
+          modglob_init := [BI_const (xx 0)] |} *)
       ];
       mod_elem := [] ;
       mod_data := [] ;
@@ -378,19 +422,41 @@ Section coroutines_client_module.
         {| imp_module := String.list_byte_of_string "coroutines module";
           imp_name := String.list_byte_of_string "par function";
           imp_desc := ID_func 1
+        |};
+        {| imp_module := String.list_byte_of_string "host";
+          imp_name := String.list_byte_of_string "a";
+          imp_desc := ID_global {| tg_mut := MUT_mut ; tg_t := T_i32 |}
+        |};
+        {| imp_module := String.list_byte_of_string "host";
+          imp_name := String.list_byte_of_string "b";
+          imp_desc := ID_global {| tg_mut := MUT_mut ; tg_t := T_i32 |}
         |}
+
       ];
-      mod_exports := [];
+      mod_exports := [
+(*        {| modexp_name := String.list_byte_of_string "a";
+          modexp_desc := MED_global (Mk_globalidx 0)
+        |} ;
+        {| modexp_name := String.list_byte_of_string "b";
+          modexp_desc := MED_global (Mk_globalidx 1)
+        |} *)
+      ];
       mod_tags := []
     |}.
 
-  Definition impts := [ET_func emptyt ; ET_func par_type].
+  Definition impts := [ET_func emptyt ; ET_func par_type;
+                       ET_glob {| tg_mut := MUT_mut ; tg_t := T_i32 |};
+                       ET_glob {| tg_mut := MUT_mut ; tg_t := T_i32 |}
+    ].
+
+  Definition expts : list extern_t := [] (* ET_glob {| tg_mut := MUT_mut ; tg_t := T_i32 |};
+                       ET_glob {| tg_mut := MUT_mut ; tg_t := T_i32 |}] *) .
 
   Lemma client_module_typing :
-    module_typing client_module impts [].
+    module_typing client_module impts expts.
   Proof.
     unfold module_typing.
-    exists [emptyt; emptyt; emptyt], (repeat {| tg_mut := MUT_mut ; tg_t := T_i32 |} 4).
+    exists [emptyt; emptyt; emptyt], (repeat {| tg_mut := MUT_mut ; tg_t := T_i32 |} 2).
     simpl.
     repeat split; eauto.
     - constructor; last constructor; last constructor; last constructor.
@@ -404,46 +470,541 @@ Section coroutines_client_module.
     - constructor; last constructor; last constructor; last constructor; last constructor.
       all: cbn; repeat split => //.
       all: constructor.
-    - constructor; last constructor; last constructor.
-      all: cbn; apply/andP; split => //.
+    - constructor; last constructor; last constructor; last constructor; last constructor.
+      all: cbn; try by apply/andP; split => //.
+      all: by apply/eqglobal_typeP.
+    (* - repeat constructor => //=.
+      unfold module_export_typing.
+      simpl. by apply/eqP.
+      unfold module_export_typing.
+      simpl. by apply/eqP. *)
   Qed.
 
 
-  Definition client_module_instantiate yield_exp_addr par_exp_addr mod_addr mod_addr' :=
+  Definition client_module_instantiate yield_exp_addr par_exp_addr a_exp_addr b_exp_addr mod_addr mod_addr' ga gb :=
     [ ID_instantiate [ yield_exp_addr ; par_exp_addr ] mod_addr [] ;
-      ID_instantiate [] mod_addr' [ yield_exp_addr ; par_exp_addr ]
+      ID_instantiate [ (* a_exp_addr ; b_exp_addr *) ] mod_addr' [ yield_exp_addr ; par_exp_addr; a_exp_addr; b_exp_addr ];
+      H_get_global ga;
+      H_get_global gb
     ].
 
   Notation "{{{{ P }}}} es {{{{ v , Q }}}}" :=
     (□ ∀ Φ, P -∗ (∀ v, Q -∗ Φ v) -∗ WP (es : host_expr) @ NotStuck ; ⊤ {{ v, Φ v }})%I (at level 50).
 
-  Lemma instantiate_client yield_exp_addr par_exp_addr mod_addr mod_addr' : 
-    
+  Lemma instantiate_client yield_exp_addr par_exp_addr a_exp_addr b_exp_addr mod_addr mod_addr' ga gb vala valb: 
+    typeof_num vala = T_i32 ->
+    typeof_num valb = T_i32 ->
     ⊢ {{{{ 
               mod_addr ↪[mods] coroutines_module ∗
                 mod_addr' ↪[mods] client_module ∗
                 (∃ exp1, yield_exp_addr ↪[vis] exp1) ∗
-                (∃ exp2, par_exp_addr ↪[vis] exp2)
+                (∃ exp2, par_exp_addr ↪[vis] exp2) ∗
+                (∃ namea, a_exp_addr ↪[vis]  {| modexp_name := namea;
+                                               modexp_desc := MED_global (Mk_globalidx ga) |}) ∗
+                (∃ nameb, b_exp_addr ↪[vis]  {| modexp_name := nameb;
+                                               modexp_desc := MED_global (Mk_globalidx gb) |}) ∗
+                (N.of_nat ga ↦[wg] {| g_mut := MUT_mut ; g_val := vala |}) ∗
+                (N.of_nat gb ↦[wg] {| g_mut := MUT_mut ; g_val := valb |}) 
+       
       }}}}
-      ((client_module_instantiate yield_exp_addr par_exp_addr mod_addr mod_addr',
-         [], empty_frame) : host_expr) 
-        {{{{  x,  ⌜x = (immHV [], empty_frame)⌝ ∗
+      ((client_module_instantiate yield_exp_addr par_exp_addr a_exp_addr b_exp_addr mod_addr mod_addr' ga gb,
+         [], empty_frame) : host_expr)
+      {{{{ x, ⌜ exists a b, x = (immHV [VAL_num (xx b); VAL_num (xx a)], empty_frame) /\ (a = 1 -> b = 1) ⌝ }}}}.
+      (* old postcond: *)
+(*        {{{{  x,  ⌜x = (immHV [], empty_frame)⌝ ∗
                          mod_addr ↪[mods] coroutines_module ∗
                          mod_addr' ↪[mods] client_module ∗
-                         ∃ inst addra addrb addrx addry vala valb valx valy addr_f1 cl_f1 addr_f2 cl_f2 addr_main cl_main,
-                           wgpt addra valb ∗
+                         ∃ addra addrb vala valb namea nameb,
+                           a_exp_addr ↪[vis] {| modexp_name := namea;
+                                               modexp_desc := MED_global (Mk_globalidx addra) |} ∗
+                             b_exp_addr ↪[vis] {| modexp_name := nameb;
+                                                 modexp_desc := MED_global (Mk_globalidx addrb) |} ∗
+
+                           wgpt addra vala ∗
                              wgpt addrb valb ∗
-                             wgpt addrx valx ∗
-                             wgpt addry valy ∗
-                             ⌜ vala = 1 -> valb = 1 ⌝ ∗
-                            N.of_nat addr_f1 ↦[wf] cl_f1 ∗
-                            N.of_nat addr_f2 ↦[wf] cl_f2 ∗
-                            N.of_nat addr_main ↦[wf] cl_main ∗
-                            
-                         
-        }}}} .
+                             ⌜ vala = 1 -> valb = 1 ⌝
+        }}}} . *)
   Proof.
+    intros Hvala Hvalb.
+    iIntros "!>" (Φ) "(Hmod1 & Hmod2 & Hexp1 & Hexp2 & [%namea Hexp3] & [%nameb Hexp4] & Hga & Hgb) HΦ".
+
+    (* instantiate coroutines module *) 
+    iApply (wp_seq_host_nostart with "[] Hmod1 [Hexp1 Hexp2]").
+    done. done.
+    2:{
+      iIntros "Hmod1".
+      iApply (instantiate_coroutines with "[$Hmod1 $Hexp1 $Hexp2]").
+      iIntros (x) "(-> & Hmod & H)".
+      iFrame.
+      instantiate (1 := λ v, (⌜ v = (immHV [], empty_frame) ⌝ ∗ _)%I).
+      iSplit; first done.
+      iExact "H".
+    }
+    by iIntros (?) "[% _]".
+    iIntros (w f) "(%Heq & %addr_yield & %addr_par & %name_yield & %name_par & %cl_yield & %cl_par & Hexp1 & Hexp2 & %Htypeyield & %Htypepar & Hwfyield & Hwfpar & #Hspecs) Hmod1".
+    iDestruct (pointsto_ne with "Hwfyield Hwfpar") as %Hne.
+    iDestruct (pointsto_ne with "Hga Hgb") as %Hne'.
+    inversion Heq; subst. clear Heq.
+
+    (* instantiate client module *)
+    iApply (instantiation_spec_operational_start_seq with "[$Hmod2 Hexp1 Hexp2 Hexp3 Hexp4 Hwfyield Hwfpar Hga Hgb]").
+    done.
+    apply client_module_typing.
+    repeat constructor.
+    by eexists [_;_].
+    1,2: by eexists [].
+    iSplitL "Hexp1 Hexp2 Hexp3 Hexp4".
+    { unfold import_resources_host.
+      instantiate (1 := [_;_;_;_]).
+      iFrame. done. }
+    iSplitL (*R "Hexp3 Hexp4"*); last first.
+    { iSplitL; last done.
+      unfold export_ownership_host.
+      iFrame. done. } 
+    unfold instantiation_resources_pre_wasm.
+    iSimpl.
+    iSplitL; last first.
+    iSplitL. by unfold module_elem_bound_check_gmap.
+    by unfold module_data_bound_check_gmap.
+    unfold import_resources_wasm_typecheck.
+    iSplitR "Hga Hgb"; last first.
+    iSplitR.
+    instantiate (1 := ∅).
+    unfold import_tab_wasm_check.
+    iSplitL.
+    by unfold import_tab_resources.
+    unfold tab_typecheck, tab_domcheck.
+    iPureIntro. split; last done. by repeat constructor.
+    iSplitR.
+    instantiate (1 := ∅).
+    unfold import_mem_wasm_check.
+    iSplitL. 
+    by unfold import_mem_resources.
+    iPureIntro.
+    split; last done.
+    by repeat constructor.
+    iSplitL.
+    instantiate (1 := <[ _ := _ ]> (<[ _ := _ ]> ∅)).
+    unfold import_glob_wasm_check.
+    iSplitL; first unfold import_glob_resources.
+    iApply big_sepM_insert; last first.
+    iFrame "Hga".
+    iApply big_sepM_insert.
+    done.
+    iFrame "Hgb". done.
+    rewrite lookup_insert_ne => //. 
+
+    iPureIntro.
+    unfold glob_typecheck, glob_domcheck.
+    simpl.
+    split; last by set_solver.
+    repeat constructor => //=.
+    rewrite lookup_insert.
+    repeat eexists => //=.
+    unfold global_agree.
+    rewrite Hvala. done.
+    rewrite lookup_insert_ne; last done.
+    rewrite lookup_insert.
+    repeat eexists => //=.
+    rewrite /global_agree /= Hvalb //.
+    unfold import_tag_wasm_check.
+    iSplitL; first by unfold import_tag_resources.
+    iPureIntro. split; last done.
+    by repeat constructor.
+    unfold import_func_wasm_check.
+    unfold import_func_resources.
+
+    instantiate (1 := (<[ _ := _ ]> (<[ _ := _]> ∅))).
+    iSplitL.
+
+    iApply big_sepM_insert.
+    2:{ iFrame "Hwfyield".
+        iApply big_sepM_insert.
+        done.
+        iFrame "Hwfpar".
+        done. }
+    rewrite lookup_insert_ne.
+    done.
+    done.
+    iPureIntro.
+    split.
+    repeat constructor => //=.
+    eexists.
+    rewrite lookup_insert.
+    split => //. 
+    by rewrite Htypeyield.
+    eexists.
+    rewrite lookup_insert_ne; last done.
+    rewrite lookup_insert.
+    split => //.
+    by rewrite Htypepar.
+    unfold func_domcheck.
+    simpl.
+    set_solver.
+    iIntros (idnstart) "H".
+    unfold instantiation_resources_post.
+    iDestruct "H" as "(Hmod2 & Himps & %inst & Hresources & Hexports)".
+    unfold module_export_resources_host.
+    iClear "Hexports".
+(*    iDestruct "Hexports" as "([%namea Hexpa] & [%nameb Hexpb] & _)".
+    simpl. *)
+    
+    unfold import_resources_host.
+    iDestruct "Himps" as "(Hexp1 & Hexp2 & _)".
+    unfold instantiation_resources_post_wasm.
+    iDestruct "Hresources" as (g_inits tab_allocs mem_allocs glob_allocs tag_allocs wts' wms') "(Himptype & %Hprefs & -> & -> & %Helembound & -> & -> & %Hdatabound & %Hinitval & -> & -> & Hresources)".
+    unfold module_glob_init_values in Hinitval.
+    unfold module_glob_init_value in Hinitval.
+    destruct Hinitval as [Hinittypes Hthose].
+    simpl in Hthose.
+    unfold those in Hthose.
+    simpl in Hthose.
+    inversion Hthose; subst.
+    unfold module_inst_resources_wasm.
+    iDestruct "Hresources" as "(Hfuncs & Htabs & Hmems & Hglobs & Htags)".
+    unfold module_inst_resources_func.
+    unfold module_inst_resources_tab.
+    unfold module_inst_resources_mem.
+    unfold module_inst_resources_glob.
+    unfold module_inst_resources_tag.
+(*    assert (exists a b c d, module_inst_global_init (module_inst_build_globals (mod_globals client_module)) g_inits = map (fun x => {| g_mut := MUT_mut ; g_val := VAL_int32 x |}) [a;b;c;d]) as (? & ? & ? & ? & ->).
+    { simpl.
+      do 4 (destruct g_inits; first by repeat eexists).
+      by repeat eexists. } *)
+(*    rewrite Heq0. *)
+    
+    destruct inst; simpl in *.
+    rewrite /get_import_func_count /get_import_table_count /get_import_mem_count
+      /get_import_global_count /get_import_tag_count /=.
+    repeat rewrite drop_0.
+    destruct inst_tags; last done.
+    destruct inst_memory; last done.
+    destruct inst_tab; last done.
+    iClear "Htags Hmems Htabs".
+
+    
+    destruct Hprefs as (-> & Hfuncpref & _ & _ & Hglobpref & _ & Hstart).
+    destruct inst_funcs; first done.
+    destruct inst_funcs; first done.
+    inversion Hfuncpref.
+    inversion H; subst.
+    clear H Hfuncpref.
+    destruct x; first done.
+    iDestruct "Hfuncs" as "[Hf1 Hfuncs]".
+    destruct x; first done.
+    iDestruct "Hfuncs" as "[Hf2 Hfuncs]".
+    destruct x; first done.
+    iDestruct "Hfuncs" as "[Hfmain Hfuncs]".
+    destruct x; last done.
+
+    destruct inst_globs; first done.
+    destruct inst_globs; first done.
+    inversion Hglobpref.
+    inversion H; subst.
+    clear H Hglobpref.
+    destruct x; first done.
+    iDestruct "Hglobs" as "[Hg1 Hglobs]".
+    destruct x; first done.
+    iDestruct "Hglobs" as "[Hg2 Hglobs]".
+    destruct x; last done.
+    
+    iClear "Hfuncs Hglobs".
+    simpl.
+    unfold check_start in Hstart.
+    move/eqP in Hstart; simpl in Hstart.
+    inversion Hstart; subst idnstart.
+    unfold import_resources_wasm_typecheck, impts.
+    iDestruct "Himptype" as "(Himpfunc & _ & _ & Himpglob & _)".
+    unfold import_func_wasm_check.
+    iDestruct "Himpfunc" as "[Himpfunc %Himpfunc]".
+    unfold import_func_resources.
+    iDestruct (big_sepM_insert with "Himpfunc") as "[Hfyield Himpfunc]".
+    rewrite lookup_insert_ne; last done.
+    done.
+    iDestruct (big_sepM_insert with "Himpfunc") as "[Hfpar _]".
+    done.
+    unfold import_func_wasm_check.
+    iDestruct "Himpglob" as "[Himpglob %Himpglob]".
+    unfold import_glob_resources.
+    iDestruct (big_sepM_insert with "Himpglob") as "[Hga Himpglob]".
+    rewrite lookup_insert_ne; last done.
+    done.
+    iDestruct (big_sepM_insert with "Himpglob") as "[Hgb Himpglob]".
+    done.
+
+    iApply wp_lift_wasm.
+
+    (* Prove the specification of main *)
+    rewrite - (app_nil_l [AI_invoke _]).
+    iApply (ewp_invoke_native with "Hfmain").
+    done. done. done.
+    iIntros "!> Hfmain".
+    iApply ewp_frame_bind.
+    done. done.
+    iSplitR; last first.
+    iSplitL "Hg1 Hg2 Hga Hgb Hf1 Hf2 Hfyield Hfpar".
+    rewrite -(app_nil_l [AI_basic _]).
+    iApply ewp_block.
+    done. done. done. done.
+    iApply (ewp_label_bind with "[-]").
+    2:{ iPureIntro.
+        instantiate (5 := []).
+        rewrite /lfilled /lfill /= app_nil_r //. }
+    rewrite (separate1 (AI_basic _)).
+    iApply ewp_seq.
+    done.
+    iSplitR; last first.
+    iSplitR.
+    iApply ewp_ref_func.
+    done.
+    auto_instantiate.
+    2: by iIntros (?) "[% _]".
+    iIntros (??) "[->->]".
+    iSimpl.
+    rewrite (separate2 (AI_ref _)).
+    iApply ewp_seq.
+    done.
+    iSplitR; last first.
+    rewrite (separate1 (AI_ref _)).
+    iSplitR.
+    iApply ewp_val_app.
+    done.
+    iSplitR; last first.
+    iApply ewp_wand.
+    iApply ewp_ref_func.
+    done.
+    auto_instantiate.
+    iIntros (??) "[->->]".
+    iSimpl.
+    auto_instantiate.
+    by iIntros "!>" (?) "[% _]".
+    2: by iIntros (?) "[% _]".
+    iIntros (??) "[->->]".
+    iSimpl.
+    rewrite (separate2 (AI_ref _)).
+    rewrite - (app_nil_r [AI_basic _]).
+    iApply ewp_wasm_empty_ctx.
+    iApply ewp_base_push.
+    done.
+    iApply ewp_call_ctx.
+    done.
+    iApply ewp_base_pull.
+    iApply ewp_wasm_empty_ctx.
+    iSimpl.
+    unfold yield_par_spec.
+    iNext. iApply fupd_ewp.
+    iMod (own_alloc Pending) as (γx) "Hγx"; first done.
+    iMod (own_alloc Pending) as (γy) "Hγy"; first done.
+    iDestruct ("Hspecs" $! P1 (P2 ga gb) (Q1 γx γy) (Q2 ga gb) (I n2 n3 γx γy))%I as (Ψ) "[Hspecyield Hspecpar]".
+    iApply (ewp_wand with "[-]").
+    iApply ("Hspecpar" with "[$] [Hga Hgb] [Hγx Hγy Hg1 Hg2] Hf1 Hf2 Hfyield").
+    { destruct vala, valb => //.
+      unfold P2, wgpt, xx.
+      iExists (Wasm_int.Z_of_uint i32m s), (Wasm_int.Z_of_uint i32m s0).
+      do 2 rewrite Wasm_int.Int32.int_of_Z_Z_of_uint.
+      iFrame. }
+    iLeft. iFrame. 
+    iIntros "!>" (f) "HP1 HI Hf1 Hfyield".
+    iApply (ewp_call_reference with "Hf1").
+    done. done.
+    iIntros "!> Hf1".
+    iApply (ewp_wand with "[-]").
+    iApply (spec_f1_proof with "[] Hf1 Hfyield HP1 HI").
+    done. iExact "Hspecyield".
+    iIntros (??) "(-> & -> & Hf1 & Hfyield & HQ1 & HI)".
+    iFrame. done.
+    iIntros "!>" (f) "HP2 HI Hf2 Hfyield".
+    iApply (ewp_call_reference with "Hf2").
+    done. done.
+    iIntros "!> Hf2".
+    iApply (ewp_wand with "[-]").
+    iApply (spec_f2_proof with "[] Hf2 Hfyield HP2 HI").
+    done. iExact "Hspecyield".
+    iIntros (??) "(-> & -> & Hf2 & Hfyield & HQ2 & HI)".
+    iFrame. done.
+    iFrame.
+    iIntros "!>" (??) "(-> & -> & HQ1 & HQ2 & HI & Hf1 & Hf2 & Hfyield & Hfpar)".
+    iIntros (LI HLI).
+    move/lfilledP in HLI; inversion HLI; subst.
+    inversion H8; subst.
+    iSimpl.
+    iApply ewp_label_value.
+    done.
+    iCombine "HQ1 HQ2 HI Hf1 Hf2 Hfyield Hfpar" as "H".
+    instantiate (1 := λ v f, (∃ γx γy, ⌜ v = immV _ ⌝ ∗ ⌜ f = Build_frame _ _ ⌝ ∗ _)%I).
+    iExists γx, γy. iSplit; first done. iSplit; first done.
+    iExact "H".
+    2: by iIntros (?) "(% & % & % & _)".
+    iIntros (??) "(%γx & %γy & -> & -> & HQ1 & HQ2 & HI & Hf1 & Hf2 & Hfyield & Hfpar)".
+    iSimpl.
+    iApply ewp_frame_value.
+    done. done.
+    iDestruct "HQ2" as (a b) "(Hga & Hgb & %Hab)".
+    iApply (wp_get_global_host with "Hga").
+    iIntros "!> !> Hga".
+    iApply (wp_get_global_host with "Hgb").
+    iIntros "!> Hgb".
+
+    
+    iApply wp_value. done.
+    iApply "HΦ".
+    iPureIntro.
+    exists a, b. split => //.
+  Qed. 
+    
       
 
-   
-     
+End coroutines_client_module.
+
+
+Section coroutines_client_adequacy.
+
+  Context (Σ: gFunctors).
+  Context {inv_preg: invGpreS Σ}.
+  Context {na_invg: na_invG Σ}.
+  Context {func_preg: gen_heapGpreS N function_closure Σ}.
+  Context {tab_preg: gen_heapGpreS (N*N) funcelem Σ}.
+  Context {tabsize_preg: gen_heapGpreS N nat Σ}.
+  Context {tablimits_preg: gen_heapGpreS N (option N) Σ}.
+  Context {mem_preg: gen_heapGpreS (N*N) byte Σ}.
+  Context {memsize_preg: gen_heapGpreS N N Σ}.
+  Context {memlimit_preg: gen_heapGpreS N (option N) Σ}.
+  Context {glob_preg: gen_heapGpreS N global Σ}.
+(*  Context {locs_preg: gen_heapGpreS unit frame Σ}. *)
+  Context {vis_preg: gen_heapGpreS N module_export Σ}.
+  Context {ms_preg: gen_heapGpreS N module Σ}.
+  Context {has_preg: gen_heapGpreS N host_action Σ}.
+  Context {tag_preg: gen_heapGpreS N function_type Σ}.
+  Context {cont_preg: gen_heapGpreS N continuation Σ}.
+  Context {one_shotg: one_shotG Σ}.
+
+  Definition near_empty_store : store_record := Build_store_record [] [] [] [] [ {| g_mut := MUT_mut; g_val := xx 0 |};  {| g_mut := MUT_mut; g_val := xx 0 |} ] [] [].
+
+  (* The following addresses could be generalised, as long as there are
+     no duplicates *)
+  Definition yield_exp_addr := 0%N.
+  Definition par_exp_addr := 1%N.
+  Definition a_exp_addr := 2%N.
+  Definition b_exp_addr := 3%N.
+
+  Definition mod_addr := 0%N.
+  Definition mod_addr' := 1%N.
+
+  Definition ga := 0.
+  Definition gb := 1.
+  
+  Definition exports: vi_store :=
+     (<[ a_exp_addr := {| modexp_name := [Byte.x00]; modexp_desc := MED_global (Mk_globalidx ga) |} ]> (
+     (<[ b_exp_addr := {| modexp_name := [Byte.x00]; modexp_desc := MED_global (Mk_globalidx gb) |} ]> (
+    (<[ yield_exp_addr := {| modexp_name := [Byte.x00]; modexp_desc := MED_global (Mk_globalidx (N.to_nat 0)) |} ]> (
+      <[ par_exp_addr := {| modexp_name := [Byte.x00]; modexp_desc := MED_global (Mk_globalidx (N.to_nat 0)) |} ]> ∅)))))).
+  
+  Lemma coroutines_client_adequacy he' S' V' M' HA':
+    rtc erased_step (([ (client_module_instantiate yield_exp_addr par_exp_addr a_exp_addr b_exp_addr mod_addr mod_addr' ga gb, [], empty_frame) ],
+                       (near_empty_store, exports, [coroutines_module; client_module], [] )) : cfg wasm_host_lang)
+      ([he'] , (S', V', M', HA')) ->
+    (forall v, iris_host.to_val he' = Some v ->
+          exists a b, v = (immHV [VAL_num (xx b); VAL_num (xx a)], empty_frame) /\ (a = 1 -> b = 1)).
+  Proof.
+    intros Hstep.
+    pose proof (wp_adequacy Σ wasm_host_lang NotStuck
+                  (client_module_instantiate yield_exp_addr par_exp_addr a_exp_addr b_exp_addr mod_addr mod_addr' ga gb, [], empty_frame)
+                  (near_empty_store, exports, [coroutines_module; client_module], [] )
+                  (λ v,  exists a b, v = (immHV [VAL_num (xx b); VAL_num (xx a)], empty_frame) /\ (a = 1 -> b = 1)) 
+      ).
+    simpl in H.
+    
+    eassert _.
+    { apply H.
+      iIntros (Hinv κs).
+      iMod (gen_heap_init (∅:gmap N function_closure)) as (func_heapg) "[Hfunc_ctx _]".
+      iMod (gen_heap_init (∅:gmap (N*N) funcelem)) as (tab_heapg) "[Htab_ctx _]".
+      iMod (gen_heap_init (∅:gmap N nat)) as (tabsize_heapg) "[Htabsize_ctx _]".
+      iMod (@gen_heap_init _ _ _ _ _ tablimits_preg (∅:gmap N (option N))) as (tablimit_heapg) "[Htablimit_ctx _]".
+      iMod (gen_heap_init (∅:gmap (N*N) byte)) as (mem_heapg) "[Hmem_ctx _]".
+      iMod (gen_heap_init (∅:gmap N N)) as (memsize_heapg) "[Hmemsize_ctx _]".
+      iMod (@gen_heap_init _ _ _ _ _ memlimit_preg (∅:gmap N (option N))) as (memlimit_heapg) "[Hmemlimit_ctx _]".
+      iMod (gen_heap_init (∅:gmap N global)) as (global_heapg) "[Hglobal_ctx _]".
+      iMod (gen_heap_init (∅: gmap N function_type)) as (tag_heapg) "[Htag_ctx _]".
+      iMod (gen_heap_init (∅: gmap N continuation)) as (cont_heapg) "[Hcont_ctx _]".
+      
+(*      apply (@gen_heapGpreS_heap) in locs_preg as frame_heapg.
+      iMod (ghost_map_alloc (∅:gmap unit frame)) as (γframe) "[Hframe_ctx _]". *)
+      apply (@gen_heapGpreS_heap) in vis_preg as vis_heapg.
+      iMod (ghost_map_alloc (∅:gmap N module_export)) as (γvis) "[Hvis_ctx _]".
+      apply (@gen_heapGpreS_heap) in ms_preg as ms_heapg.
+      iMod (ghost_map_alloc (∅:gmap N module)) as (γms) "[Hms_ctx _]".
+      apply (@gen_heapGpreS_heap) in has_preg as has_heapg.
+      iMod (ghost_map_alloc (∅:gmap N host_action)) as (γhas) "[Hhas_ctx _]".
+
+      iMod (@na_alloc Σ na_invg) as (logrel_nais) "Hna".
+      pose wasmg := WasmG Σ Hinv func_heapg cont_heapg tag_heapg tab_heapg tabsize_heapg
+                          tablimit_heapg mem_heapg memsize_heapg memlimit_heapg
+                          global_heapg.
+      pose visgg := HVisG Σ vis_heapg γvis.
+      pose msgg := HMsG Σ ms_heapg γms.
+      pose hasgg := HAsG Σ has_heapg γhas.
+      pose logrel_na_invs := Build_logrel_na_invs _ na_invg logrel_nais.
+(*      pose proof (instantiate_client yield_exp_addr par_exp_addr a_exp_addr b_exp_addr mod_addr mod_addr'). *)
+
+      iMod (ghost_map_insert par_exp_addr {| modexp_name := [Byte.x00]; modexp_desc := MED_global (Mk_globalidx (N.to_nat 0)) |}
+             with "Hvis_ctx") as "[Hvis_ctx Hv1]";[auto|].
+      iMod (ghost_map_insert yield_exp_addr {| modexp_name := [Byte.x00]; modexp_desc := MED_global (Mk_globalidx (N.to_nat 0)) |}
+             with "Hvis_ctx") as "[Hvis_ctx Hv2]";[auto|].
+      iMod (ghost_map_insert b_exp_addr {| modexp_name := [Byte.x00]; modexp_desc := MED_global (Mk_globalidx gb) |}
+             with "Hvis_ctx") as "[Hvis_ctx Hv3]";[auto|].
+      iMod (ghost_map_insert a_exp_addr {| modexp_name := [Byte.x00]; modexp_desc := MED_global (Mk_globalidx ga) |}
+             with "Hvis_ctx") as "[Hvis_ctx Hv4]";[auto|].
+      iMod (ghost_map_insert mod_addr coroutines_module with "Hms_ctx") as "[Hms_ctx Hm0]";[auto|].
+      iMod (ghost_map_insert mod_addr' client_module with "Hms_ctx") as "[Hms_ctx Hm1]";[auto|].
+      
+      iMod (gen_heap_alloc _ (N.of_nat ga) {| g_mut := MUT_mut; g_val := xx 0 |} with "Hglobal_ctx") as "[Hglobal_ctx [Hg _]]";[auto|].
+      iMod (gen_heap_alloc _ (N.of_nat gb) {| g_mut := MUT_mut; g_val := xx 0 |} with "Hglobal_ctx") as "[Hglobal_ctx [Hg' _]]";[auto|].
+
+      iDestruct (instantiate_client $! (λ v, ⌜ exists a b, v = (immHV [VAL_num (xx b); VAL_num (xx a)], empty_frame) /\ (a = 1 -> b = 1) ⌝%I) 
+                  with "[$Hm1 $Hm0 Hv1 Hv2 Hv3 Hv4 Hg Hg']") as "HH".
+      3:{ iSplitL "Hv2"; first by iFrame.
+          iSplitL "Hv1"; first by iFrame.
+          iSplitL "Hv4"; first by iFrame.
+          iSplitL "Hv3"; first by iFrame.
+          iFrame.
+      }
+      done. done.
+
+      iDestruct ("HH" with "[]") as "HH";[auto|].
+      iModIntro.
+      iExists _,_. iFrame "HH". iFrame. }
+    intros v Hval.
+    destruct X. eapply adequate_result with (t2 := []).
+    apply iris_host.of_to_val in Hval as <-. eauto.
+  Qed.
+
+End coroutines_client_adequacy.
+
+Theorem coroutines_example he' S' V' M' HA':
+    rtc erased_step (([ (client_module_instantiate yield_exp_addr par_exp_addr a_exp_addr b_exp_addr mod_addr mod_addr' ga gb, [], empty_frame) ],
+                       (near_empty_store, exports, [coroutines_module; client_module], [] )) : cfg wasm_host_lang)
+      ([he'] , (S', V', M', HA')) ->
+    (forall v, iris_host.to_val he' = Some v ->
+          exists a b, v = (immHV [VAL_num (xx b); VAL_num (xx a)], empty_frame) /\ (a = 1 -> b = 1)).
+Proof.
+   set (Σ := #[invΣ;
+              na_invΣ;
+              gen_heapΣ N function_closure;
+              gen_heapΣ (N*N) funcelem;
+              gen_heapΣ N nat;
+              gen_heapΣ N (option N);
+              gen_heapΣ (N*N) byte;
+              gen_heapΣ N N;
+              gen_heapΣ N (option N);
+              gen_heapΣ N global;
+              gen_heapΣ N module_export;
+              gen_heapΣ N module;
+               gen_heapΣ N host_action;
+               gen_heapΣ N function_type;
+               gen_heapΣ N continuation;
+               one_shotΣ
+      ]).
+  eapply (@coroutines_client_adequacy Σ); typeclasses eauto.
+Qed.
+
